pulse/lib/pulse/lib/Pulse.Lib.Primitives.fsti
@@ -51,17 +51,17 @@ val cas (r:ref U32.t) (u v:U32.t) (#i:erased U32.t)
 
 val read_atomic_box (r:B.box U32.t) (#n:erased U32.t) (#p:perm)
   : stt_atomic U32.t emp_inames
-    (B.pts_to r #p n)
-    (fun x -> B.pts_to r #p n ** pure (reveal n == x))
+    (pts_to r #p n)
+    (fun x -> pts_to r #p n ** pure (reveal n == x))
 
 val write_atomic_box (r:B.box U32.t) (x:U32.t) (#n:erased U32.t)
   : stt_atomic unit emp_inames
-        (B.pts_to r n) 
-        (fun _ -> B.pts_to r (hide x))
+        (pts_to r n) 
+        (fun _ -> pts_to r (hide x))
 
 val cas_box (r:B.box U32.t) (u v:U32.t) (#i:erased U32.t)
   : stt_atomic bool #Observable emp_inames 
-    (B.pts_to r i)
+    (pts_to r i)
     (fun b ->
-      cond b (B.pts_to r v ** pure (reveal i == u)) 
-             (B.pts_to r i))
+      cond b (pts_to r v ** pure (reveal i == u)) 
+             (pts_to r i))
